This is up through hello-world.

examples/hello-world/Makefile.ml
@@ -1,0 +1,25 @@
+ROOT=./../..
+
+OCAMLC=ocamlc.opt
+OCAMLOPT=ocamlopt.opt
+
+EXEC=`basename \`pwd\``
+
+COMPFLAGS=-I ./ml -I .extract -I $(ROOT)/src/ml/
+
+EXTRACTED=$(wildcard .extract/*.ml)
+
+ml: main.byte main.native
+
+main.byte: $(ROOT)/src/ml/ynot.cma ml/main.cmo $(EXTRACTED:%.ml=%.cmo)
+	ocamlc $(COMPFLAGS) -o main.byte $(ROOT)/src/ml/ynot.cma .extract/*.cmo ml/main.cmo
+
+main.native: $(ROOT)/src/ml/ynot.cmxa ml/main.cmx  $(EXTRACTED:%.ml=%.cmx)
+	ocamlopt.opt $(COMPFLAGS) -o main.native $(ROOT)/src/ml/ynot.cmxa .extract/*.cmx ml/main.cmx
+
+clean:
+	rm -f main.byte main.native
+	rm -f ml/*.cmo ml/*.cmi ml/*.cmx
+
+include ../Makefile.ynot
+include .depend
