src/ml/BasisImpl.ml
@@ -1,0 +1,9 @@
+open STImpl
+
+(** printString : string -> unit sTsep **)
+let axiom_printString str () = 
+  print_string (MlCoq.list_ascii_to_string str); flush stdout
+
+(** printStringLn : string -> unit sTsep **)
+let axiom_printStringLn str () = 
+  print_string (MlCoq.list_ascii_to_string str); print_string "\r\n"; flush stdout
