src/ml/MlCoq.ml
@@ -1,0 +1,48 @@
+(** Coq Extraction Definitions **)
+type ascii =
+  | Ascii of bool * bool * bool * bool * bool * bool * bool * bool
+
+type nat =
+  | O
+  | S of nat
+
+(** Helpful functions **)
+let int_to_nat =
+  let rec f i acc =
+    if i = 0 then 
+      acc
+    else
+      f (i - 1) (S acc)
+  in 
+  fun i -> 
+    if i < 0 then 
+      failwith "iton : negative number!"
+    else 
+      f i O
+;;
+
+let nat_to_int =
+  let rec f acc n =
+    match n with
+    | O -> acc
+    | S m -> f (1 + acc) m
+  in
+  f 0
+;;
+
+let ascii_to_char asc = 
+  let Ascii (a, b, c, d, e, f, g, h) = asc in
+  let bits : bool list = [a;b;c;d;e;f;g;h] in
+  let ch = List.fold_right (fun v a -> a * 2 + if v then 1 else 0) bits 0 in
+  Char.chr ch
+;;
+
+let list_ascii_to_string s = 
+  let rec r s =
+    match s with
+      [] -> ""
+    | first :: rest ->
+	(String.make 1 (ascii_to_char first)) ^ (r rest)
+  in r s
+;;
+  
