src/ml/STImpl.ml
@@ -1,0 +1,28 @@
+open Obj;;
+
+type 'a axiom_ST = unit -> 'a ;;
+
+let axiom_STBind b k = fun () -> let v = b () in k v ();;
+
+let axiom_STReturn v () = v ;;
+
+let axiom_STContra () = failwith "ST Contradiction" ;;
+
+let axiom_STWeaken x = x ;;
+
+let axiom_STStrengthen x = x ;;
+ 
+let axiom_STNew v = fun () -> ref (Obj.magic v) ;;
+
+let axiom_STFree p = fun () -> () ;;
+
+let axiom_STRead p = fun () -> Obj.obj !p ;;
+
+let axiom_STWrite p v = fun () -> (p := Obj.repr v) ;;
+
+(** ((a -> (unit -> b)) -> a -> (unit -> b)) -> a -> (unit -> b) **)
+let axiom_STFix f x = fun () -> 
+  let rec fix g = fun a -> f (fix f) a
+  in (fix f) x () ;;
+
+let exec io = io ()
