examples/hello-world/Extract.v
@@ -1,0 +1,5 @@
+Require Import Ynot.Extract.
+
+Require HelloWorld.
+
+Extraction ".extract/HelloWorld.ml" HelloWorld.main.
