examples/hello-world/HelloWorld.v
@@ -1,0 +1,11 @@
+Require Import Ynot.
+Require Import Basis.
+Require Import String.
+
+Open Local Scope string_scope.
+Open Local Scope stsepi_scope.
+
+Definition main : STsep (__) (fun _:unit => hprop_empty).
+   refine (printStringLn "Hello World");
+   sep fail auto.
+Qed.
